Charge!/src/Charge/Rewriter/BIlogicRewrite.v
@@ -1,34 +1,132 @@
-Require Import MirrorCore.Lambda.Expr.
-Require Import MirrorCore.Views.FuncView.
-Require Import MirrorCore.Reify.ReifyClass.
+Require Import ExtLib.Core.RelDec.
+Require Import ExtLib.Data.POption.
 
+Require Import MirrorCore.Lambda.Ptrns.
+Require Import MirrorCore.Lemma.
+Require Import MirrorCore.TCLemma.
+Require Import MirrorCore.PLemma.
+Require Import MirrorCore.Polymorphic.
+Require Import MirrorCore.Views.Ptrns.
+Require Import MirrorCore.Views.FuncView.
+Require Import MirrorCore.Reify.Reify.
+Require Import MirrorCore.Reify.ReifyView.
+Require Import MirrorCore.RTac.RTac.
+
+Require Import MirrorCore.Lambda.RewriteRelations.
+Require Import MirrorCore.Lambda.Rewrite.Respectful.
+Require Import MirrorCore.Lambda.Rewrite.Core.
+Require Import MirrorCore.Lambda.Rewrite.HintDbs.
+Require Import MirrorCore.Lambda.Rewrite.Repeat.
+Require Import MirrorCore.Lambda.Rewrite.BottomUp.
+Require Import MirrorCore.Lambda.Rewrite.Reduce.
+Require Import MirrorCore.Lambda.Rewrite.Rewrite.
+Require Import MirrorCore.Lambda.Rewrite.Tactic.
+Require Import MirrorCore.Lambda.PolyInst.
+
+Require Import MirrorCore.CTypes.CTypeUnify.
+Require Import MirrorCore.CTypes.CoreTypes.
+Require Import MirrorCore.CTypes.BaseType.
+
+Require Import ChargeCore.Logics.ILogic.
 Require Import ChargeCore.Logics.BILogic.
 
+Require Import Charge.Views.ILogicView.
+Require Import Charge.Patterns.ILogicPattern.
+Require Import Charge.Reify.ILogicReify.
 Require Import Charge.Views.BILogicView.
 Require Import Charge.Patterns.BILogicPattern.
+Require Import Charge.Reify.BILogicReify.
+Require Import Charge.Rewriter.ILogicRewrite.
+Require Import Charge.Tactics.Rtac.PApply.
 
-Section ReifyBILogic.
-  Context {typ func : Set} {FV : PartialView func (bilfunc typ)}.
-  Context {t : Reify typ}.
+Section RewriteBILogic.
+  Context {typ' : nat -> Set} {func : Set}.
 
-  Definition reify_emp : Command (expr typ func) :=
-    CPattern (ls := (typ:Type)::nil)
-             (RApp (RApp (RExact (@empSP)) (RGet 0 RIgnore)) RIgnore)
-             (fun (x : function (CCall (reify_scheme typ))) => mkEmp x).
+  Notation typ := (ctyp typ').   
+  
+  Context {RType_typ : RType typ}.
+  Context {RSym_func : RSym func}.
+  Context {RelDec_eq_typ : RelDec (@eq typ)}.
+  Context {Expr_expr : Expr typ (expr typ func)}.
+  Context {Typ2_tyArr : Typ2 _ RFun}.
+  Context {Typ2Ok_tyArr : Typ2Ok Typ2_tyArr}.
+  Context {Typ0_tyProp : Typ0 _ Prop}.
+  Context {FVIL : PartialView func (ilfunc typ)}.
+  Context {FVBIL : PartialView func (bilfunc typ)}.
+  Context {FV_typ : PartialView typ (base_typ 0)}.
+  
+  Context {bilops : @bilogic_ops typ RType_typ}.
+                        
+  Let tyProp : typ := @typ0 _ _ _ Typ0_tyProp.
+  Let tyArr : typ -> typ -> typ := @typ2 _ _ _ Typ2_tyArr.
 
-  Definition reify_star : Command (expr typ func) :=
-    CPattern (ls := (typ:Type)::nil)
-             (RApp (RApp (RExact (@sepSP)) (RGet 0 RIgnore)) RIgnore)
-             (fun (x : function (CCall (reify_scheme typ))) => Inj (fStar x)).
+  Existing Instance Reify_typ.
+              
+  Local Instance Reify_expr : Reify (expr typ func) :=
+    Reify_func_no_table typ func 
+      (reify_plogic typ func :: 
+       reify_ilogic typ func :: 
+       reify_bilogic typ func :: nil).
 
-  Definition reify_wand : Command (expr typ func) :=
-    CPattern (ls := (typ:Type)::nil)
-             (RApp (RApp (RExact (@wandSP)) (RGet 0 RIgnore)) RIgnore)
-             (fun (x : function (CCall (reify_scheme typ))) => Inj (fWand x)).
+  Definition bil_ignore := 
+    RApp (RExact (@BILogicOps)) RIgnore :: 
+    RApp (RApp (RApp (RExact (@BILogic)) RIgnore) RIgnore) RIgnore :: 
+    il_ignore.
+    
+  Definition lem_typ x := ptc_lem_typ typ (expr typ func) (expr typ func) x bil_ignore.
+  Definition rel_lem_typ x := ptc_rel_lem_typ typ func (expr typ func) x bil_ignore.
+  Definition proper_rel_lem_typ x := ptc_proper_rel_lem_typ typ func (expr typ func) x bil_ignore.
+    
+  Definition lem_bilexistsscL1 : rel_lem_typ 2 :=
+    Eval unfold Lemma.add_var, Lemma.add_prem, Lemma.vars, Lemma.concl, 
+                Lemma.premises, List.app in
+      <:: @bilexistsscL1 ::>.
+              
+  Definition lem_bilexistsscR1 : rel_lem_typ 2 :=
+    Eval unfold Lemma.add_var, Lemma.add_prem, Lemma.vars, Lemma.concl, 
+                Lemma.premises, List.app in
+      <:: @bilexistsscR1 ::>.
+              
+  Definition lem_bilexistsscL2 : rel_lem_typ 2 :=
+    Eval unfold Lemma.add_var, Lemma.add_prem, Lemma.vars, Lemma.concl, 
+                Lemma.premises, List.app in
+      <:: @bilexistsscL2 ::>.
+              
+  Definition lem_bilexistsscR2 : rel_lem_typ 2 :=
+    Eval unfold Lemma.add_var, Lemma.add_prem, Lemma.vars, Lemma.concl, 
+                Lemma.premises, List.app in
+      <:: @bilexistsscR2 ::>.
+              
+  Definition lem_Proper_sc : proper_rel_lem_typ 1 :=
+    Eval unfold Lemma.add_var, Lemma.add_prem, Lemma.vars, Lemma.concl, 
+                Lemma.premises in
+    <:: @sepSP_lentails_m ::>.
+  
+  Definition is_bilogic1 : polymorphic typ 1 bool := 
+  	fun t => 
+   	  match bilops t with
+      | pSome _ => true
+      | _ => false
+      end.
+      
+  Definition is_bilogic2 : polymorphic typ 2 bool := 
+  	fun t _ => 
+   	  match bilops t with
+      | pSome _ => true
+      | _ => false
+      end.
+      
+  Definition pull_exists_lemmasL : RewriteHintDb (expr typ func) :=
+    @PRw_tc _ _ _ 2 lem_bilexistsscL1 is_bilogic2 (runOnGoals IDTAC) ::
+    @PRw_tc _ _ _ 2 lem_bilexistsscL2 is_bilogic2 (runOnGoals IDTAC) :: nil.
 
-  Definition reify_bilogic : Command (expr typ func) :=
-    CFirst (reify_emp :: reify_star :: reify_wand :: nil).
+  Definition pull_exists_lemmasR : RewriteHintDb (expr typ func) :=
+    @PRw_tc _ _ _ 2 lem_bilexistsscR1 is_bilogic2 (runOnGoals IDTAC) :: 
+    @PRw_tc _ _ _ 2 lem_bilexistsscR1 is_bilogic2 (runOnGoals IDTAC) :: nil.
 
-End ReifyBILogic.
+  Definition bil_proper : ProperDb (expr typ func) :=
+    (@PPr_tc typ func (expr typ func) 1 (pconcl lem_Proper_sc) is_bilogic1 :: 
+     @PPr_tc typ func (expr typ func) 1 (pconcl (flip_proper_rel_lem lem_Proper_sc)) is_bilogic1 ::
+     nil).
 
-Arguments reify_bilogic _ _ {_ _}.
+End RewriteBILogic.
