Charge!/src/Charge/Rewriter/ILogicRewrite.v
@@ -1,7 +1,9 @@
 Require Import ExtLib.Core.RelDec.
+Require Import ExtLib.Data.POption.
 
 Require Import MirrorCore.Lambda.Ptrns.
 Require Import MirrorCore.Lemma.
+Require Import MirrorCore.PLemma.
 Require Import MirrorCore.TCLemma.
 Require Import MirrorCore.PLemma.
 Require Import MirrorCore.Polymorphic.
@@ -9,11 +11,17 @@ Require Import MirrorCore.Views.Ptrns.
 Require Import MirrorCore.Views.FuncView.
 Require Import MirrorCore.Reify.Reify.
 Require Import MirrorCore.Reify.ReifyView.
+Require Import MirrorCore.RTac.RTac.
 
 Require Import MirrorCore.Lambda.RewriteRelations.
 Require Import MirrorCore.Lambda.Rewrite.Respectful.
 Require Import MirrorCore.Lambda.Rewrite.Core.
 Require Import MirrorCore.Lambda.Rewrite.HintDbs.
+Require Import MirrorCore.Lambda.Rewrite.Repeat.
+Require Import MirrorCore.Lambda.Rewrite.BottomUp.
+Require Import MirrorCore.Lambda.Rewrite.Reduce.
+Require Import MirrorCore.Lambda.Rewrite.Rewrite.
+Require Import MirrorCore.Lambda.Rewrite.Tactic.
 Require Import MirrorCore.Lambda.PolyInst.
 
 Require Import MirrorCore.CTypes.CTypeUnify.
@@ -25,16 +33,7 @@ Require Import ChargeCore.Logics.ILogic.
 Require Import Charge.Views.ILogicView.
 Require Import Charge.Patterns.ILogicPattern.
 Require Import Charge.Reify.ILogicReify.
-
-Section IgnoreILogic.
-
-  Definition reify_ILogicOps : RPattern :=
-    RApp (RExact (@ILogicOps)) RIgnore.
-  
-  Definition reify_ILogic : RPattern  :=
-    RApp (RApp (RExact (@ILogic)) RIgnore) RIgnore.
- 
-End IgnoreILogic.
+Require Import Charge.Tactics.Rtac.PApply.
 
 Section RewriteILogic.
   Context {typ' : nat -> Set} {func : Set}.
@@ -44,51 +43,31 @@ Section RewriteILogic.
   Context {RType_typ : RType typ}.
   Context {RSym_func : RSym func}.
   Context {RelDec_eq_typ : RelDec (@eq typ)}.
-  Context {RelDec_eq_func : RelDec (@eq func)}.
   Context {Expr_expr : Expr typ (expr typ func)}.
   Context {Typ2_tyArr : Typ2 _ RFun}.
   Context {Typ2Ok_tyArr : Typ2Ok Typ2_tyArr}.
   Context {Typ0_tyProp : Typ0 _ Prop}.
   Context {FV : PartialView func (ilfunc typ)}.
   Context {FV_typ : PartialView typ (base_typ 0)}.
-      
+  
+  Context {ilops : @logic_ops typ RType_typ}.
+  Context (unify_func : PolyInst.sym_unifier (typ := typ) (sym := func)).
+                        
   Let tyProp : typ := @typ0 _ _ _ Typ0_tyProp.
   Let tyArr : typ -> typ -> typ := @typ2 _ _ _ Typ2_tyArr.
-(* 
-  Definition RbaseD (e : expr typ func) (t : typ) : option (TypesI.typD t -> TypesI.typD t -> Prop) :=
-    castD option (RFun (typD t) (RFun (typD t) Prop)) (env_exprD nil nil (tyArr t (tyArr t tyProp)) e).
 
-
-  Theorem RbaseD_single_type
-  : forall (r : expr typ func) (t1 t2 : typ)
-           (rD1 : TypesI.typD t1 -> TypesI.typD t1 -> Prop)
-           (rD2 : TypesI.typD t2 -> TypesI.typD t2 -> Prop),
-      RbaseD r t1 = Some rD1 -> RbaseD r t2 = Some rD2 -> t1 = t2.
-  Proof.
-    unfold RbaseD, env_exprD, castD. simpl; intros.
-    unfold eq_sym in *. simpl in *.
-    
-    generalize (lambda_exprD_deterministic _ _ _ H0 H). unfold Rty.
-    intros. inversion H3. reflexivity.
-  Qed.  
- 
- 
-  Fixpoint from_terms (rs : list (expr typ func) : refl_dec Rbase :=
-    match rs with
-    | nil => fun _ => false
-    | r :: rs => fun r' =>
-      if expr_eq_dec _ _ r r' then true else from_terms rs r'
-    end.
-*)
- 
   Definition is_refl : refl_dec (expr typ func) :=
    	run_ptrn
-      (pmap (fun _ => true) (inj (ptrn_view _ (fptrnEntails ignore))))
+      (pmap (fun _ => true) 
+        (inj (por (ptrn_view _ (fptrnEntails ignore))
+                  (ptrn_view _ (fptrnImpl ignore)))))
       false.
     
   Definition is_trans : trans_dec (expr typ func) :=
    	run_ptrn 
-      (pmap (fun _ => true) (inj (ptrn_view _ (fptrnEntails ignore))))
+      (pmap (fun _ => true) 
+        (inj (por (ptrn_view _ (fptrnEntails ignore))
+                  (ptrn_view _ (fptrnImpl ignore)))))
       false.
     
   Local Instance Reify_typ : Reify typ :=
@@ -96,79 +75,162 @@ Section RewriteILogic.
 
   Local Instance Reify_expr : Reify (expr typ func) :=
     Reify_func_no_table typ func (reify_plogic typ func :: reify_ilogic typ func :: nil).
-
-  Definition lem_typ x := 
-    polymorphic typ x 
-      (tc_lemma typ (expr typ func) 
-         (rw_concl typ func (expr typ func))
-         (RApp (RExact (@ILogicOps)) RIgnore :: 
-          RApp (RApp (RExact (@ILogic)) RIgnore) RIgnore :: 
-          nil)).  
-
-  Definition proper_lem_typ x := 
-    polymorphic typ x
-      (tc_lemma typ (expr typ func)
-        (Proper_concl typ func (expr typ func))
-         (RApp (RExact (@ILogicOps)) RIgnore :: 
-          RApp (RApp (RExact (@ILogic)) RIgnore) RIgnore :: 
-          nil)).  
-                      
-  Definition lem_landexistsDL : lem_typ 2 :=
-    Eval unfold Lemma.add_var, Lemma.add_prem , Lemma.vars , Lemma.concl , Lemma.premises, List.app in
-      <:: @landexistsDL ::>.
+                
+  Definition il_ignore := 
+    RApp (RExact (@ILogicOps)) RIgnore :: 
+    RApp (RApp (RExact (@ILogic)) RIgnore) RIgnore :: 
+    nil.
+    
+  Definition lem_typ x := ptc_lem_typ typ (expr typ func) (expr typ func) x il_ignore.
+  Definition rel_lem_typ x := ptc_rel_lem_typ typ func (expr typ func) x il_ignore.
+  Definition proper_rel_lem_typ x := ptc_proper_rel_lem_typ typ func (expr typ func) x il_ignore.
+  
+  Definition flip_rw_concl (c : rw_concl typ func (expr typ func)) :=
+    Build_rw_concl (lhs c) (Rflip'' (rel c)) (rhs c). 
+                  
+  Definition flip_Proper_concl (c : Proper_concl typ func (expr typ func)) :=
+    mkProper (Rflip'' (relation c)) (term c). 
+                  
+  Definition flip_rel_lem {x : nat} (l : rel_lem_typ x) : rel_lem_typ x :=
+    fmap_polymorphic (fun x => mkLemma (vars x) (premises x) (flip_rw_concl (concl x))) l.
+  
+  Definition flip_proper_rel_lem {x : nat} (l : proper_rel_lem_typ x) : proper_rel_lem_typ x :=
+    fmap_polymorphic (fun x => mkLemma (vars x) (premises x) (flip_Proper_concl (concl x))) l.
+  
+  Definition lem_landexistsDL1 : rel_lem_typ 2 :=
+    Eval unfold Lemma.add_var, Lemma.add_prem, Lemma.vars, Lemma.concl, 
+                Lemma.premises, List.app in
+      <:: @landexistsDL1 ::>.
               
-  Definition lem_landexistsDR : lem_typ 2 :=
-    Eval unfold Lemma.add_var, Lemma.add_prem , Lemma.vars , Lemma.concl , Lemma.premises, List.app in
-      <:: @landexistsDR ::>.
+  Definition lem_landexistsDR1 : rel_lem_typ 2 :=
+    Eval unfold Lemma.add_var, Lemma.add_prem, Lemma.vars, Lemma.concl, 
+                Lemma.premises, List.app in
+      <:: @landexistsDR1 ::>.
                             
-  Definition lem_lorexistsDR : lem_typ 2 :=
-    Eval unfold Lemma.add_var, Lemma.add_prem , Lemma.vars , Lemma.concl , Lemma.premises, List.app in
-      <:: @landexistsDR ::>.
+  Definition lem_landexistsDL2 : rel_lem_typ 2 :=
+    Eval unfold Lemma.add_var, Lemma.add_prem, Lemma.vars, Lemma.concl, 
+                Lemma.premises, List.app in
+      <:: @landexistsDL2 ::>.
               
-  Definition lem_Proper_exists : proper_lem_typ 2 :=
-    Eval unfold Lemma.add_var, Lemma.add_prem , Lemma.vars , Lemma.concl , Lemma.premises in
+  Definition lem_landexistsDR2 : rel_lem_typ 2 :=
+    Eval unfold Lemma.add_var, Lemma.add_prem, Lemma.vars, Lemma.concl, 
+                Lemma.premises, List.app in
+      <:: @landexistsDR2 ::>.
+                            
+  Definition lem_lorexistsDR : rel_lem_typ 2 :=
+    Eval unfold Lemma.add_var, Lemma.add_prem, Lemma.vars, Lemma.concl, 
+                Lemma.premises, List.app in
+      <:: @lorexistsDR ::>.
+              
+  Definition lem_Proper_exists : proper_rel_lem_typ 2 :=
+    Eval unfold Lemma.add_var, Lemma.add_prem, Lemma.vars, Lemma.concl, 
+                Lemma.premises, function in
     <:: @lexists_lentails_m ::>.
 
-  Definition lem_Proper_forall : proper_lem_typ 2 :=
-    Eval unfold Lemma.add_var, Lemma.add_prem , Lemma.vars , Lemma.concl , Lemma.premises in
+  Definition lem_Proper_forall : proper_rel_lem_typ 2 :=
+    Eval unfold Lemma.add_var, Lemma.add_prem , Lemma.vars , Lemma.concl , 
+                Lemma.premises, function in
     <:: @lforall_lentails_m ::>.
 
-  Definition lem_Proper_and : proper_lem_typ 1 :=
-    Eval unfold Lemma.add_var, Lemma.add_prem , Lemma.vars , Lemma.concl , Lemma.premises in
+  Definition lem_Proper_and : proper_rel_lem_typ 1 :=
+    Eval unfold Lemma.add_var, Lemma.add_prem, Lemma.vars, Lemma.concl, 
+                Lemma.premises in
     <:: @land_lentails_m ::>.
 
-  Definition lem_Proper_or : proper_lem_typ 1 :=
-    Eval unfold Lemma.add_var, Lemma.add_prem , Lemma.vars , Lemma.concl , Lemma.premises in
+  Definition lem_Proper_or : proper_rel_lem_typ 1 :=
+    Eval unfold Lemma.add_var, Lemma.add_prem, Lemma.vars, Lemma.concl, 
+                Lemma.premises in
     <:: @lor_lentails_m ::>.
 
-  Definition lem_Proper_impl : proper_lem_typ 1 :=
-    Eval unfold Lemma.add_var, Lemma.add_prem , Lemma.vars , Lemma.concl , Lemma.premises in
+  Definition lem_Proper_impl : proper_rel_lem_typ 1 :=
+    Eval unfold Lemma.add_var, Lemma.add_prem, Lemma.vars, Lemma.concl, 
+                Lemma.premises in
     <:: @limpl_lentails_m ::>.
 
-  Fixpoint polymorphic_map {A B : Set} {x : nat} (f : A -> B) : polymorphic typ x A -> polymorphic typ x B :=
-    match x with
-    | 0 => fun a => f a
-    | S x => fun a x => polymorphic_map f (a x)
-    end.
-
-Arguments concl {_ _ _} _.
-
-  Definition lentails_respectful : ResolveProper typ func (expr typ func) :=
-    do_prespectful (Rbase := expr typ func) rel_dec tyVar (type_sym_unifier (CTypeUnify.ctype_unify_slow _))
-      (@PPr typ func (expr typ func) 2 (polymorphic_map concl lem_Proper_exists) ::
-       @PPr typ func (expr typ func) 2 (polymorphic_map concl lem_Proper_forall) ::
-       @PPr typ func (expr typ func) 1 (polymorphic_map concl lem_Proper_and) ::
-       @PPr typ func (expr typ func) 1 (polymorphic_map concl lem_Proper_or) ::
-       @PPr typ func (expr typ func) 1 (polymorphic_map concl lem_Proper_impl) ::
-       nil).
-
+  Definition lem_Proper_entails : proper_rel_lem_typ 1 :=
+    Eval unfold Lemma.add_var, Lemma.add_prem, Lemma.vars, Lemma.concl, 
+                Lemma.premises, function in
+    <:: @lentails_lentails_m ::>.
+  
   Definition lem_entails_refl : lem_typ 1 :=
-    Eval unfold Lemma.add_var, Lemma.add_prem, Lemma.vars, Lemma.concl, Lemma.premises, List.app in
+    Eval unfold Lemma.add_var, Lemma.add_prem, Lemma.vars, Lemma.concl, 
+         Lemma.premises, List.app, function in
       <:: @lentails_refl ::>.
 
-  Definition the_lemmas : RewriteHintDb (expr typ func) :=
-    @PRw _ _ _ 1 lem_pull_ex_and_left DO_REFL ::
-    @PRw _ _ _ 1 lem_pull_ex_and_right DO_REFL ::
+  Definition is_ilogic1 : polymorphic typ 1 bool := 
+  	fun t => 
+   	  match ilops t with
+      | pSome _ => true
+      | _ => false
+      end.
+      
+  Definition is_ilogic2 : polymorphic typ 2 bool := 
+  	fun t _ => 
+   	  match ilops t with
+      | pSome _ => true
+      | _ => false
+      end.
+      
+  Definition plem_entails_refl : PolyLemma typ (expr typ func) (expr typ func) :=
+    {| p_n := 1;
+       p_lem := lem_entails_refl;
+       p_tc := is_ilogic1 |}.
 
-Check (or_respectful lentails_respectful lentails_respectful).
+  Definition DO_REFL :=
+    (runOnGoals (THEN (TRY INSTANTIATE) (runOnGoals (TRY (PAPPLY unify_func plem_entails_refl))))).
+
+  Definition pull_exists_lemmasL : RewriteHintDb (expr typ func) :=
+    @PRw_tc _ _ _ 2 lem_landexistsDL1 is_ilogic2 (runOnGoals IDTAC) ::
+    @PRw_tc _ _ _ 2 lem_landexistsDL2 is_ilogic2 (runOnGoals IDTAC) :: nil.
+
+  Definition pull_exists_lemmasR : RewriteHintDb (expr typ func) :=
+    @PRw_tc _ _ _ 2 lem_landexistsDR1 is_ilogic2 (runOnGoals IDTAC) :: 
+    @PRw_tc _ _ _ 2 lem_landexistsDR2 is_ilogic2 (runOnGoals IDTAC) :: 
+    @PRw_tc _ _ _ 2 lem_lorexistsDR is_ilogic2 (runOnGoals IDTAC) :: nil.
+
+  Definition get_respectful (pdb : ProperDb (expr typ func)) : 
+    ResolveProper typ func (expr typ func) :=
+    do_prespectful expr_eqb tyVar unify_func
+      (@PPr_tc typ func (expr typ func) 2 (pconcl lem_Proper_exists) is_ilogic2 ::
+       @PPr_tc typ func (expr typ func) 2 (pconcl (flip_proper_rel_lem lem_Proper_exists)) is_ilogic2 ::
+       @PPr_tc typ func (expr typ func) 1 (pconcl lem_Proper_entails) is_ilogic1 :: 
+       @PPr_tc typ func (expr typ func) 1 (pconcl (flip_proper_rel_lem lem_Proper_entails)) is_ilogic1 :: 
+       @PPr_tc typ func (expr typ func) 1 (pconcl lem_Proper_or) is_ilogic1 :: 
+       @PPr_tc typ func (expr typ func) 1 (pconcl (flip_proper_rel_lem lem_Proper_or)) is_ilogic1 :: 
+       @PPr_tc typ func (expr typ func) 1 (pconcl lem_Proper_impl) is_ilogic1 :: 
+       @PPr_tc typ func (expr typ func) 1 (pconcl (flip_proper_rel_lem lem_Proper_impl)) is_ilogic1 :: 
+       @PPr_tc typ func (expr typ func) 1 (pconcl lem_Proper_and) is_ilogic1 ::
+       @PPr_tc typ func (expr typ func) 1 (pconcl (flip_proper_rel_lem lem_Proper_and)) is_ilogic1 :: pdb).
+
+  Definition simple_reduce (e : expr typ func) : expr typ func :=
+    run_ptrn
+      (pmap (fun abcd => let '(a,(b,(c,d),e)) := abcd in
+                         App a (Abs c (App (App b d) e)))
+            (app get (abs get (fun t =>
+                                 app (app get
+                                          (pmap (fun x => (t,Red.beta x)) get))
+                                     (pmap Red.beta get)))))
+    e e.
+    
+  Definition rw_lemmas (lems : RewriteHintDb (expr typ func)) : 
+    RwAction typ func (expr typ func) :=
+    rw_post_simplify simple_reduce (rw_simplify Red.beta (using_prewrite_db expr_eqb (CompileHints unify_func lems))).
+  
+  Definition rw_action
+  	(rdb : RewriteHintDb (expr typ func)) 
+  	(rp : ResolveProper typ func (expr typ func)) : RwAction typ func (expr typ func) :=
+    repeat_rewrite (fun e r =>
+                      bottom_up (is_reflR is_refl) (is_transR is_trans) (rw_lemmas rdb) 
+                                 rp e r)
+                   (is_reflR is_refl) (is_transR is_trans) false 300.
+
+  Definition REWRITE 
+  	(rdb : RewriteHintDb (expr typ func)) 
+  	(pdb : ProperDb (expr typ func)) : rtac typ (expr typ func) :=
+    let rp := get_respectful pdb in
+    let rw := rw_action rdb rp in
+        @auto_setoid_rewrite_bu typ func (expr typ func)
+                            (Rflip (Rinj (Inj (fImpl tyProp))))
+                            (is_reflR is_refl) (is_transR is_trans) rw rp.
+
 End RewriteILogic.
