Charge!/src/Charge/Tactics/Rtac/Red.v
@@ -1,0 +1,54 @@
+Require Import Charge.Views.ILogicView.
+Require Import Charge.Patterns.ILogicPattern.
+Require Import Charge.Views.BILogicView.
+Require Import Charge.Patterns.BILogicPattern.
+Require Import Charge.Views.EmbedView.
+Require Import Charge.Patterns.EmbedPattern.
+
+Require Import MirrorCore.Lambda.ExprCore.
+Require Import MirrorCore.CTypes.CoreTypes.
+Require Import MirrorCore.Views.Ptrns.
+Require Import MirrorCore.Lib.ApplicativeView.
+Require Import MirrorCore.RTac.RTac.
+
+Section Red.
+  Context {typ' : nat -> Set} {func : Set}.
+  Context {TSym_typ' : TSym typ'}.
+  Let typ := ctyp typ'.
+  Local Instance RType_typ : RType typ := RType_ctyp typ' _.
+  Local Instance Typ2_typ : Typ2 RType_typ RFun := Typ2_Fun.
+  Local Instance Typ0_Prop : Typ0 RType_typ Prop := Typ0_Prop _ _.
+  Context {FVIL : PartialView func (ilfunc typ)}.
+  Context {FVBIL : PartialView func (bilfunc typ)}.
+  Context {FVEmbed : PartialView func (embed_func typ)}.
+  Context {FVAp : PartialView func (ap_func typ)}.
+  Context {Expr_expr : Expr typ (expr typ func)}.
+
+  Definition pointwise_redF (f : typ -> expr typ func -> expr typ func) : 
+    ptrn (expr typ func) (expr typ func)  :=
+    Eval compute in 
+      por (bil_pointwise_red f (fun x => x)) 
+          (por (embed_pointwise_red f (fun x => x)) 
+               (por (red_ap_ptrn f)
+                    (il_pointwise_red f (fun x => x)))).
+
+  Fixpoint pointwise_red_aux (s : expr typ func) (t : typ) (e : expr typ func) {struct e} : expr typ func :=
+    run_ptrn (pointwise_redF (pointwise_red_aux s)) (App e s) e.
+
+  Definition pointwise_red (s e : expr typ func) := pointwise_red_aux s tyProp e.
+
+  Definition red_entails_lhs :=
+    pmap (fun t' => let '(t, (p, s), r) := t' in 
+    		 mkEntails t (pointwise_red s p) r)
+         (ptrnEntails get (Ptrns.app get get) get).
+
+  Definition RED_ENTAILS : rtac typ (expr typ func) :=
+    fun c s e =>
+      run_ptrn (pmap (fun e => More s (GGoal e)) red_entails_lhs) Fail e.
+      
+  Lemma RED_ENTAILS_sound : rtac_sound RED_ENTAILS.
+  Proof.
+    admit.
+  Admitted.
+
+End Red.
